Diff/Galois.v
@@ -7,23 +7,23 @@ Unset Printing Implicit Defensive.
 Require Import ClassicalExtras.
 Require Import MyNotation.
 
-Definition monotone {X Y : Set} (f : (X -> Prop) -> (Y -> Prop)) : Prop :=
+Definition monotone {X Y : Type} (f : (X -> Prop) -> (Y -> Prop)) : Prop :=
   forall (π1 π2: X -> Prop), (π1 ⊆ π2) -> (f π1 ⊆ f π2).
 
-Definition idempotent {X : Set} (f : (X -> Prop) -> (X -> Prop)) : Prop :=
+Definition idempotent {X : Type} (f : (X -> Prop) -> (X -> Prop)) : Prop :=
   forall π: X -> Prop, f (f π) = f π.
 
-Definition extensive {X : Set} (f : (X -> Prop) -> (X -> Prop)) : Prop :=
+Definition extensive {X : Type} (f : (X -> Prop) -> (X -> Prop)) : Prop :=
   forall π: X -> Prop, π ⊆ (f π).
 
 
-Definition lift {X Y : Set} (f :(X -> Prop) -> (Y -> Prop))
+Definition lift {X Y : Type} (f :(X -> Prop) -> (Y -> Prop))
                             (H : (X -> Prop) -> Prop) : ((Y -> Prop) -> Prop) :=
   fun (b1 : Y -> Prop) => exists b2, (H b2) /\ b1 = f b2.
 
 (* Definition of the adjunction law *)
 
-Definition Adjunction_law {A C : Set}
+Definition Adjunction_law {A C : Type}
            (α : (C -> Prop) -> (A -> Prop))
            (γ : (A -> Prop) -> (C -> Prop)) :=
   forall (a: A -> Prop) (c: C -> Prop),  (α c) ⊆ a <-> c ⊆ (γ a).
@@ -32,24 +32,24 @@ Definition Adjunction_law {A C : Set}
 (* We define Galois connection between powersets ordered by set inclusion:
      (2^X, ⊆) ⇆ (2^Y, ⊆)
    *)
-Structure Galois_Connection (A C : Set) := {
+Structure Galois_Connection (A C : Type) := {
     α : (C -> Prop) -> (A -> Prop);
     γ : (A -> Prop) -> (C -> Prop);
     adjunction_law : Adjunction_law α γ
   }.
 
 
-Definition Galois_fst {A C : Set}
+Definition Galois_fst {A C : Type}
            (α: (C -> Prop) -> (A -> Prop))
            (γ: (A -> Prop) -> (C -> Prop)) :=
   forall (c: C -> Prop),  c ⊆ (γ (α c)).
 
-Definition Galois_snd {A C : Set}
+Definition Galois_snd {A C : Type}
            (α: (C -> Prop) -> (A -> Prop))
            (γ: (A -> Prop) -> (C -> Prop)) :=
   forall (a : A -> Prop), (α (γ a)) ⊆ a.
 
-Lemma Galois_equiv {A C: Set}
+Lemma Galois_equiv {A C: Type}
       (α: (C -> Prop) -> (A -> Prop))
       (γ: (A -> Prop) -> (C -> Prop)) :
   Adjunction_law α γ <-> ( monotone α /\ monotone γ /\ Galois_fst α γ  /\ Galois_snd α γ).
@@ -69,12 +69,12 @@ Proof.
 Qed.
 
 
-Definition Insertion_snd {A C : Set}
+Definition Insertion_snd {A C : Type}
            (α: (C -> Prop) -> (A -> Prop))
            (γ: (A -> Prop) -> (C -> Prop)) :=
   forall (a : A -> Prop), (α (γ a)) = a.
 
-Structure Galois_Insertion (A C : Set) := {
+Structure Galois_Insertion (A C : Type) := {
             α__i : (C -> Prop) -> (A -> Prop);
             γ__i : (A -> Prop) -> (C -> Prop);
             mono_α : monotone α__i;
@@ -84,7 +84,7 @@ Structure Galois_Insertion (A C : Set) := {
           }.
 
 
-Lemma Insertion_coercion_Connection {A C : Set} :
+Lemma Insertion_coercion_Connection {A C : Type} :
   Galois_Insertion A C -> Galois_Connection A C.
 Proof.
   move => [α γ mono_alpha mono_gamma H1 H2].
@@ -101,15 +101,15 @@ Coercion Insertion_coercion_Connection  : Galois_Insertion >-> Galois_Connection
      between (2^C, ⊆) and (2^A, ⊆).
    *)
 
-Definition low_rel  {A C : Set} (rel : C -> A -> Prop) : (C -> Prop) -> (A -> Prop) :=
+Definition low_rel  {A C : Type} (rel : C -> A -> Prop) : (C -> Prop) -> (A -> Prop) :=
   fun (c : C -> Prop) =>
     (fun (x : A) => exists (y : C), (c y) /\ rel y x).
 
-Definition up_rel {A C : Set} (rel : C -> A -> Prop) : (A -> Prop) -> (C -> Prop) :=
+Definition up_rel {A C : Type} (rel : C -> A -> Prop) : (A -> Prop) -> (C -> Prop) :=
   fun (a : A -> Prop) =>
     (fun (y : C) => forall (x : A), (rel y x -> a x)).
 
-Lemma induced_adj_law {A C : Set} (rel : C -> A -> Prop) :
+Lemma induced_adj_law {A C : Type} (rel : C -> A -> Prop) :
   Adjunction_law (low_rel rel) (up_rel rel).
 Proof.
   move => a c. rewrite /low_rel /up_rel. split.
@@ -117,12 +117,12 @@ Proof.
                                                + move => H x [y [c_y rel_y_x]]. by apply: (H y).
 Qed.
 
-Definition induced_connection {A C : Set} (rel : C -> A -> Prop) : Galois_Connection A C :=
+Definition induced_connection {A C : Type} (rel : C -> A -> Prop) : Galois_Connection A C :=
   Build_Galois_Connection (induced_adj_law rel).
 
 
 (** *upper closure operator  \cite{giacobazzi2018abstract} (pag 7) *)
-Record Uco {X: Set} :=
+Record Uco {X: Type} :=
   {
     uco: (X -> Prop) -> (X -> Prop);
     mono: monotone uco;
