Diff/LanguageModel.v
@@ -7,9 +7,9 @@ Require Import MyNotation.
 
 Record Language := {
 
-   prg : Set; (* Whole programs *)
-   par : Set; (* Partial programs *)
-   ctx : Set; (* Contexts *)
+   prg : Type; (* Whole programs *)
+   par : Type; (* Partial programs *)
+   ctx : Type; (* Contexts *)
    plug : par -> ctx -> prg (* Linking operation *)
 
    }.
@@ -17,7 +17,7 @@ Record Language := {
 
 (* CA: semantics of a language can be defined over an arbitrary set *)
 
-Record Semantics (L : Language) (trace_set : Set) := {
+Record Semantics (L : Language) (trace_set : Type) := {
 
   sem : prg L -> trace_set -> Prop;
   non_empty_sem : forall W, exists t, sem W t
@@ -26,19 +26,19 @@ Record Semantics (L : Language) (trace_set : Set) := {
 
 
 Definition beh {L : Language}
-               {trace_set : Set}
+               {trace_set : Type}
                (S : Semantics L trace_set)
                (W : prg L) : prop trace_set :=
   fun t => sem S W t.
 
 Definition sat {L : Language}
-               {trace_set : Set}
+               {trace_set : Type}
                (S : Semantics L trace_set)
                (W : prg L) (π : prop trace_set) : Prop :=
   forall t, sem S W t -> π t.
 
 Lemma sat_upper_closed  {L : Language}
-                        {trace_set : Set}
+                        {trace_set : Type}
                         (S : Semantics L trace_set)
                         (W : prg L ) (π1 π2 : prop trace_set) :
   sat S W π1 -> π1 ⊆ π2 -> sat S W π2.
@@ -50,19 +50,19 @@ Qed.
 
 
 Definition hsat{L : Language}
-               {trace_set : Set}
+               {trace_set : Type}
                (S : Semantics L trace_set)
                (W : prg L) (H : hprop trace_set) : Prop :=
   H (beh S W).
 
 Definition rsat {L : Language}
-                {trace_set : Set}
+                {trace_set : Type}
                 (S : Semantics L trace_set)
                 (P : par L) (π : prop trace_set) : Prop :=
   forall C, sat S (plug L P C) π.
 
 Lemma rsat_upper_closed {L : Language}
-                        {trace_set : Set}
+                        {trace_set : Type}
                         (S : Semantics L trace_set)
                         (P : par L ) (π1 π2 : prop trace_set) :
   rsat S P π1 -> π1 ⊆ π2 -> rsat S P π2.
@@ -73,13 +73,13 @@ Proof.
 Qed.
 
 Definition rhsat  {L : Language}
-                  {trace_set : Set}
+                  {trace_set : Type}
                   (S : Semantics L trace_set)
                   (P : par L) (H : hprop trace_set) : Prop :=
   forall C, hsat S (plug L P C) H.
 
 Lemma neg_sat  {L : Language}
-               {trace_set : Set}
+               {trace_set : Type}
                {S : Semantics L trace_set} :
   forall (W : prg L) (π : prop trace_set),
     ~ sat S W π <-> exists t, sem S W t /\ ~ π t.
@@ -92,7 +92,7 @@ Qed.
 
 (* Considering moving these two lemmas to a separate module *)
 Lemma neg_rsat {L : Language}
-               {trace_set : Set}
+               {trace_set : Type}
                (S : Semantics L trace_set) :
   forall (P : par L) (π : prop trace_set),
     (~ rsat S P π <->
@@ -109,7 +109,7 @@ Proof.
 Qed.
 
 Lemma neg_rhsat {L : Language}
-                {trace_set : Set}
+                {trace_set : Type}
                 (S : Semantics L trace_set) :
   forall P H,  (~ rhsat S P H <-> ( exists (C : ctx L), ~ H (beh S ( plug L P C )))).
 Proof.
